This commit was manufactured by cvs2svn to create tag 'V8-0pl3'.
git-svn-id: svn://scm.gforge.inria.fr/svnroot/coq-contribs/tags/V8-0pl3@329 0cf17b13-060f-0410-b1b1-c666bec9822a

FSetAVL.v
@@ -1,3 +1,4 @@
+
 (***********************************************************************)
 (*  v      *   The Coq Proof Assistant  /  The Coq Development Team    *)
 (* <O___,, *        INRIA-Rocquencourt  &  LRI-CNRS-Orsay              *)
@@ -273,7 +274,7 @@ Module Make (X: OrderedType) <: Sdep with Module E := X.
     end.
 
   Definition max (x y : Z) : Z :=
-    if Z_lt_ge_dec x y then fun _ => y else fun _ => x.
+    if Z_lt_ge_dec x y then y else x.
 
   (** Instead of writing [h = 1 + (max (height l) (height r))] we prefer 
       the following relation [height_of_node l r h] to ease the use of 
@@ -3169,6 +3170,272 @@ Module Make (X: OrderedType) <: Sdep with Module E := X.
     right; apply lt_not_eq; auto.
     left; auto.
     right; intro; apply (lt_not_eq s' s); auto; apply eq_sym; auto.
+  Defined.
+
+
+  (** A new comparison algorithm suggested by Xavier Leroy:
+
+type enumeration = End | More of elt * t * enumeration
+
+let rec cons s e = match s with
+  | Empty -> e
+  | Node(l, v, r, _) -> cons l (More(v, r, e))
+
+let rec compare_aux e1 e2 = match (e1, e2) with
+  | (End, End) -> 0
+  | (End, More _) -> -1
+  | (More _, End) -> 1
+  | (More(v1, r1, k1), More(v2, r2, k2)) ->
+      let c = Ord.compare v1 v2 in
+      if c <> 0 then c else compare_aux (cons r1 k1) (cons r2 k2)
+
+let compare s1 s2 = compare_aux (cons s1 End) (cons s2 End)
+*)
+
+  (** ** Enumeration of the elements of a tree *)
+
+  Inductive enumeration : Set :=
+   | End : enumeration
+   | More : elt -> tree -> enumeration -> enumeration.
+
+  (** [flatten_e e] returns the list of elements of [e] i.e. the list
+      of elements actually compared *)
+ 
+   Fixpoint flatten_e (e : enumeration) : list elt :=
+    match e with
+    | End => []
+    | More x t r => x :: elements_tree t ++ flatten_e r
+    end.
+
+  (** [sorted_e e] expresses that elements in the enumeration [e] are
+      sorted, and that all trees in [e] are binary search trees. *)
+
+  Inductive In_tree_e (x:elt) : enumeration -> Prop :=
+    | InEHd1 :
+        forall (y : elt) (s : tree) (e : enumeration),
+        X.eq x y -> In_tree_e x (More y s e)
+    | InEHd2 :
+        forall (y : elt) (s : tree) (e : enumeration),
+        In_tree x s -> In_tree_e x (More y s e)
+    | InETl :
+        forall (y : elt) (s : tree) (e : enumeration),
+        In_tree_e x e -> In_tree_e x (More y s e).
+
+  Hint Constructors In_tree_e.
+
+  Inductive sorted_e : enumeration -> Prop :=
+    | SortedEEnd : sorted_e End
+    | SortedEMore :
+        forall (x : elt) (s : tree) (e : enumeration),
+        bst s ->
+        (gt_tree x s) ->
+        sorted_e e ->
+        (forall y : elt, In_tree_e y e -> X.lt x y) ->
+        (forall y : elt,
+         In_tree y s -> forall z : elt, In_tree_e z e -> X.lt y z) ->
+        sorted_e (More x s e).
+
+  Hint Constructors sorted_e.
+
+  Lemma in_flatten_e :
+   forall (x : elt) (e : enumeration), L.ME.In x (flatten_e e) -> In_tree_e x e.
+  Proof.
+    simple induction e; simpl in |- *; intuition.
+    inversion_clear H.
+    inversion_clear H0; auto.
+    elim (in_app x _ _ H1); auto.
+  Qed.
+
+  Lemma sorted_flatten_e :
+   forall e : enumeration, sorted_e e -> L.ME.Sort (flatten_e e).
+  Proof.
+    simple induction e; simpl in |- *; intuition.
+    apply cons_sort.
+    apply sort_app; inversion H0; auto.
+    intros; apply H8; auto.
+    apply in_flatten_e; auto.
+    apply L.ME.Inf_In.
+    inversion_clear H0.
+    intros; elim (in_app_or _ _ _ H0); intuition.
+    apply H2; auto.
+    apply H4; apply in_flatten_e; auto.
+  Qed.
+
+  (** key lemma for correctness *)
+
+  Lemma flatten_e_elements :
+    forall (x : elt) (l r : tree) (z : Z) (e : enumeration),
+    elements_tree l ++ flatten_e (More x r e) =
+    elements_tree (Node l x r z) ++ flatten_e e.
+  Proof.
+    intros; simpl.
+    apply compare_flatten_1.
+  Qed.
+
+  (** termination of [compare_aux] *)
+ 
+  Fixpoint measure_e_t (s : tree) : Z :=
+    match s with
+    | Leaf => 0
+    | Node l _ r _ => 1 + measure_e_t l + measure_e_t r
+    end.
+
+  Fixpoint measure_e (e : enumeration) : Z :=
+    match e with
+    | End => 0
+    | More _ s r => 1 + measure_e_t s + measure_e r
+    end.
+
+  Ltac Measure_e_t := unfold measure_e_t in |- *; fold measure_e_t in |- *.
+  Ltac Measure_e := unfold measure_e in |- *; fold measure_e in |- *.
+
+  Lemma measure_e_t_0 : forall s : tree, measure_e_t s >= 0.
+  Proof.
+    simple induction s.
+    simpl in |- *; omega.
+    intros.
+    Measure_e_t; omega. (* BUG Simpl! *)
+  Qed.
+
+  Ltac Measure_e_t_0 s := generalize (measure_e_t_0 s); intro.
+
+  Lemma measure_e_0 : forall e : enumeration, measure_e e >= 0.
+  Proof.
+    simple induction e.
+    simpl in |- *; omega.
+    intros.
+    Measure_e; Measure_e_t_0 t0; omega.
+  Qed.
+
+  Ltac Measure_e_0 e := generalize (measure_e_0 e); intro.
+
+  (** Induction principle over the sum of the measures for two lists *)
+
+  Definition compare2_rec2 :
+    forall P : enumeration -> enumeration -> Set,
+    (forall x x' : enumeration,
+     (forall y y' : enumeration,
+      measure_e y + measure_e y' < measure_e x + measure_e x' -> P y y') ->
+     P x x') -> forall x x' : enumeration, P x x'.
+  Proof.
+    intros P H x x'.
+    apply
+     well_founded_induction_type_2
+      with
+        (R := fun yy' xx' : enumeration * enumeration =>
+              measure_e (fst yy') + measure_e (snd yy') <
+              measure_e (fst xx') + measure_e (snd xx')); 
+     auto.                      
+    apply
+     Wf_nat.well_founded_lt_compat
+      with
+        (f := fun xx' : enumeration * enumeration =>
+              Zabs_nat (measure_e (fst xx') + measure_e (snd xx'))).
+    intros; apply Zabs.Zabs_nat_lt.
+    Measure_e_0 (fst x0); Measure_e_0 (snd x0); Measure_e_0 (fst y);
+     Measure_e_0 (snd y); intros; omega.
+  Qed.
+
+  (** [cons t e] adds the elements of tree [t] on the head of 
+      enumeration [e]. Code:
+ 
+  let rec cons s e = match s with
+  | Empty -> e
+  | Node(l, v, r, _) -> cons l (More(v, r, e))
+  *)
+
+  Definition cons :
+    forall (s : tree) (e : enumeration),
+    bst s ->
+    sorted_e e ->
+    (forall (x y : elt), In_tree x s -> In_tree_e y e -> X.lt x y) ->
+    { r : enumeration 
+    | sorted_e r /\ 
+      measure_e r = measure_e_t s + measure_e e /\
+      flatten_e r = elements_tree s ++ flatten_e e
+      (* forall (x : elt), In_tree_e x r <-> (In_tree x s \/ In_tree_e x e) *)
+    }.
+  Proof.
+    simple induction s; intuition.
+    (* s = Leaf *)
+    exists e; intuition.
+    (* s = Node t0 t1 t2 z *)
+    clear H0.
+    case (H (More t1 t2 e)); clear H; intuition.
+    inversion_clear H1; auto.
+    constructor; inversion_clear H1; auto.
+    inversion_clear H0; intuition.
+    inversion_clear H1.
+    apply ME.lt_eq with t1; auto.
+    inversion_clear H1.
+    apply X.lt_trans with t1; auto.
+    exists x; intuition.
+    generalize H4; Measure_e; intros; Measure_e_t; omega.
+    rewrite H5.
+    apply flatten_e_elements.
+  Defined.
+
+  Definition compare2_aux :
+    forall e1 e2 : enumeration,
+    sorted_e e1 ->
+    sorted_e e2 ->
+    Compare L.lt L.eq (flatten_e e1) (flatten_e e2).
+  Proof.
+    intros e1 e2; pattern e1, e2 in |- *; apply compare2_rec2.
+    simple destruct x; simple destruct x'; intuition.
+    (* x = x' = End *)
+    constructor 2; unfold L.eq, L.Equal in |- *; intuition.
+    (* x = End x' = More *)
+    constructor 1; simpl in |- *; auto.
+    (* x = More x' = End *)
+    constructor 3; simpl in |- *; auto.
+    (* x = More e t0 e0, x' = More e3 t1 e4 *)
+    case (X.compare e e3); intro.
+    (* e < e3 *)
+    constructor 1; simpl; auto.
+    (* e = e3 *)
+    case (cons t0 e0).
+    inversion_clear H0; auto.
+    inversion_clear H0; auto.
+    inversion_clear H0; auto.
+    intro c1; intuition.
+    case (cons t1 e4).
+    inversion_clear H1; auto.
+    inversion_clear H1; auto.
+    inversion_clear H1; auto.
+    intro c2; intuition.
+    case (H c1 c2); clear H; intuition.
+    Measure_e; omega.
+    constructor 1; simpl.
+    apply L.lt_cons_eq; auto.
+    rewrite H5 in l; rewrite H8 in l; auto.
+    constructor 2; simpl.
+    apply l_eq_cons; auto.
+    rewrite H5 in e6; rewrite H8 in e6; auto.
+    constructor 3; simpl.
+    apply L.lt_cons_eq; auto.
+    rewrite H5 in l; rewrite H8 in l; auto.
+    (* e > e3 *)
+    constructor 3; simpl; auto.
+  Defined.
+
+  Definition compare2 : forall s1 s2 : t, Compare lt eq s1 s2.
+  Proof.
+    intros (s1, s1_bst, s1_avl) (s2, s2_bst, s2_avl); unfold lt, eq in |- *;
+     simpl in |- *.
+    case (cons s1 End); intuition.
+    inversion_clear H0.
+    case (cons s2 End); intuition.
+    inversion_clear H3.
+    simpl in H2; rewrite <- app_nil_end in H2.
+    simpl in H5; rewrite <- app_nil_end in H5.
+    case (compare2_aux x x0); intuition.
+    constructor 1; simpl in |- *.
+    rewrite H2 in l; rewrite H5 in l; auto.
+    constructor 2; apply L_eq_eq; simpl in |- *.
+    rewrite H2 in e; rewrite H5 in e; auto.
+    constructor 3; simpl in |- *.
+    rewrite H2 in l; rewrite H5 in l; auto.
   Defined.
 
   Write State "toto".
